WIP: Proof for gcm_encrypt wrapper

vale/code/arch/x64/interop/GCMencryptOpt_stdcalls.fst
@@ -198,6 +198,7 @@ val gcm128_encrypt_opt':
     )
 
 
+inline_for_extraction
 let gcm128_encrypt_opt' key auth_b auth_bytes auth_num keys_b iv_b hkeys_b abytes_b
   in128x6_b out128x6_b len128x6 in128_b out128_b len128_num inout_b plain_num scratch_b tag_b =
   
@@ -332,9 +333,9 @@ val gcm128_encrypt_opt_alloca:
 
       B.live h0 scratch_b /\ B.live h0 inout_b /\ B.live h0 abytes_b /\
 
-      B.length auth_b = UInt64.v auth_len /\
+      B.length auth_b = (UInt64.v auth_len / 16) * 16 /\
       B.length iv_b = 16 /\
-      B.length plain_b = UInt64.v plain_len /\
+      B.length plain_b = (UInt64.v plain_len / 16) * 16 /\
       B.length out_b = B.length plain_b /\
       B.length hkeys_b = 160 /\
       B.length tag_b == 16 /\
@@ -359,11 +360,89 @@ val gcm128_encrypt_opt_alloca:
                   (B.loc_union (B.loc_buffer iv_b)
                   (B.loc_union (B.loc_buffer scratch_b)
                   (B.loc_union (B.loc_buffer out_b)
-                  (B.loc_buffer inout_b))))) h0 h1      
+                  (B.loc_buffer inout_b))))) h0 h1 /\
+      (length_aux4 iv_b;
+       DV.length_eq (get_downview iv_b);
+       let iv_LE = low_buffer_read TUInt8 TUInt128 h0 iv_b 0 in
+       let iv_BE = reverse_bytes_quad32 iv_LE in
+       let ctr_BE_1 = Mkfour 1 iv_BE.lo1 iv_BE.hi2 iv_BE.hi3 in
+       let ctr_BE_2 = Mkfour 2 iv_BE.lo1 iv_BE.hi2 iv_BE.hi3 in
+       let plain_d = get_downview plain_b in
+       DV.length_eq (get_downview plain_b);
+       length_aux3 plain_b (UInt64.v plain_len / 16);       
+       let plain_u = UV.mk_buffer plain_d Views.up_view128 in
+       let inout_d = get_downview inout_b in
+       length_aux3 inout_b 1;      
+       let inout_u = UV.mk_buffer inout_d Views.up_view128 in       
+       let out_d = get_downview out_b in
+       length_aux3 out_b (UInt64.v plain_len / 16); 
+       DV.length_eq (get_downview out_b);
+       let out_u = UV.mk_buffer out_d Views.up_view128 in
+       let plain_in =
+         if (UInt64.v plain_len > B.length plain_b) then
+           Seq.append (UV.as_seq h0 plain_u) (UV.as_seq h0 inout_u)
+         else UV.as_seq h0 plain_u
+       in let cipher_out =
+         if (UInt64.v plain_len > B.length plain_b) then
+           Seq.append (UV.as_seq h1 out_u)
+                      (UV.as_seq h1 inout_u)
+         else UV.as_seq h1 out_u in
+       
+       DV.length_eq (get_downview hkeys_b);
+       let h = reverse_bytes_quad32 (low_buffer_read TUInt8 TUInt128 h1 hkeys_b 0) in
+       let length_quad = reverse_bytes_quad32 (Mkfour (8 * UInt64.v plain_len) 0 (8 * UInt64.v auth_len) 0) in
+       let auth_d = get_downview auth_b in
+       length_aux3 auth_b (UInt64.v auth_len / 16);
+       let auth_u = UV.mk_buffer auth_d Views.up_view128 in
+       let abytes_d = get_downview abytes_b in
+       length_aux3 abytes_b 1;      
+       let abytes_u = UV.mk_buffer abytes_d Views.up_view128 in        
+       let cipher_bytes =
+         if UInt64.v plain_len > B.length plain_b then
+           UV.as_seq h1 inout_u
+         else Seq.empty
+       in let auth_in =
+         if UInt64.v auth_len > (UInt64.v auth_len / 16) * 128 / 8 then
+           Seq.append (Seq.append (Seq.append (Seq.append
+             (UV.as_seq h0 auth_u) (UV.as_seq h0 abytes_u))
+             (UV.as_seq h1 out_u))
+             cipher_bytes)
+             (Seq.create 1 length_quad)
+         else
+           Seq.append (Seq.append (Seq.append
+             (UV.as_seq h0 auth_u) (UV.as_seq h1 out_u))
+             cipher_bytes)
+             (Seq.create 1 length_quad)
+       in
+       DV.length_eq (get_downview tag_b);
+       low_buffer_read TUInt8 TUInt128 h1 tag_b 0 ==
+         gctr_encrypt_block ctr_BE_1 (ghash_LE h auth_in) AES_128 (Ghost.reveal key) 0 /\
+       gctr_partial AES_128 (B.length plain_b / 16 + 1) plain_in cipher_out (Ghost.reveal key) ctr_BE_2       
+       )
     )
 
+let lemma_uv_split (h:HS.mem) (b:uint8_p) (n:UInt32.t) : Lemma
+  (requires B.length b % 16 = 0 /\ UInt32.v n % 16 = 0 /\ UInt32.v n <= B.length b)
+  (ensures (
+    let b1 = B.gsub b 0ul n in
+    let b2 = B.gsub b n (UInt32.uint_to_t (B.length b) - n) in
+    let b1_d = get_downview b1 in
+    length_aux3 b1 (B.length b1 / 16);
+    let b1_u = UV.mk_buffer b1_d Views.up_view128 in
+    let b2_d = get_downview b2 in
+    length_aux3 b2 (B.length b2 / 16);    
+    let b2_u = UV.mk_buffer b2_d Views.up_view128 in
+    let b_d = get_downview b in
+    length_aux3 b (B.length b / 16);    
+    let b_u = UV.mk_buffer b_d Views.up_view128 in       
+    let split_bs = Seq.append (UV.as_seq h b1_u) (UV.as_seq h b2_u) in
+    let bs = UV.as_seq h b_u in
+    Seq.equal bs split_bs)
+  ) = admit()
 
-let gcm128_encrypt_opt_alloca key plain_b plain_len auth_b auth_len iv_b
+
+inline_for_extraction
+let gcm128_encrypt_opt_alloca key plain_b plain_len auth_b auth_bytes iv_b
   out_b tag_b keys_b hkeys_b scratch_b inout_b abytes_b =
 
   let h0 = get() in
@@ -371,76 +450,375 @@ let gcm128_encrypt_opt_alloca key plain_b plain_len auth_b auth_len iv_b
   // Compute length of biggest blocks of 6 * 128-bit blocks
   let len128x6 = UInt64.mul (plain_len / 96uL) 96uL in
   if len128x6 / 16uL >= 18uL then (
+
     // Compute the size of the remaining 128-bit blocks
     let len128_num = ((plain_len / 16uL) * 16uL) - len128x6 in
-    let auth_num = (auth_len / 16uL) * 16uL in
     // Casting to uint32 is here the equality
     FStar.Math.Lemmas.small_mod (UInt64.v len128x6) pow2_32;
     FStar.Math.Lemmas.small_mod (UInt64.v len128_num) pow2_32;
-    FStar.Math.Lemmas.small_mod (UInt64.v auth_num) pow2_32;
     let in128x6_b = B.sub plain_b 0ul (uint64_to_uint32 len128x6) in
     let out128x6_b = B.sub out_b 0ul (uint64_to_uint32 len128x6) in
+    assume (UInt32.v (uint64_to_uint32 len128x6) + UInt32.v (uint64_to_uint32 len128_num) <= B.length plain_b);
     let in128_b = B.sub plain_b (uint64_to_uint32 len128x6) (uint64_to_uint32 len128_num) in
     let out128_b = B.sub out_b (uint64_to_uint32 len128x6) (uint64_to_uint32 len128_num) in
-    let vauth_b = B.sub auth_b 0ul (uint64_to_uint32 auth_num) in
+
+    length_aux3 in128x6_b (UInt64.v len128x6 / 16);
+    assume (B.length in128_b = 16 * (UInt64.v len128_num / 16));
+    length_aux3 in128_b (UInt64.v len128_num / 16);
+    length_aux3 out128x6_b (UInt64.v len128x6 / 16);
+    length_aux3 out128_b (UInt64.v len128_num / 16);
+    length_aux3 inout_b 1;
+    length_aux3 plain_b (UInt64.v plain_len / 16);
+    length_aux3 out_b (UInt64.v plain_len / 16);
+
+    let auth_num = UInt64.div auth_bytes 16uL in
+    let len128x6' = UInt64.div len128x6 16uL in
+    let len128_num' = UInt64.div len128_num 16uL in
 
     gcm128_encrypt_opt'
       key
-      vauth_b 
-      auth_len 
-      (UInt64.div auth_num 16uL) 
+      auth_b 
+      auth_bytes
+      auth_num
       keys_b 
       iv_b 
       hkeys_b 
       abytes_b 
       in128x6_b
       out128x6_b 
-      (UInt64.div len128x6 16uL)
+      len128x6'
       in128_b
       out128_b
-      (UInt64.div len128_num 16uL)
+      len128_num'
       inout_b
       plain_len 
       scratch_b
-      tag_b
+      tag_b;
+
+    let h1 = get() in
+
+    assert (
+      length_aux4 iv_b;
+       DV.length_eq (get_downview iv_b);
+       let iv_LE = low_buffer_read TUInt8 TUInt128 h0 iv_b 0 in
+       let iv_BE = reverse_bytes_quad32 iv_LE in
+       let ctr_BE_1 = Mkfour 1 iv_BE.lo1 iv_BE.hi2 iv_BE.hi3 in    
+       let out128x6_d = get_downview out128x6_b in
+       length_aux3 out128x6_b (UInt64.v len128x6');
+       let out128x6_u = UV.mk_buffer out128x6_d Views.up_view128 in
+       let out128_d = get_downview out128_b in
+       length_aux3 out128_b (UInt64.v len128_num');
+       let out128_u = UV.mk_buffer out128_d Views.up_view128 in      
+       let inout_d = get_downview inout_b in
+       length_aux3 inout_b 1;      
+       let inout_u = UV.mk_buffer inout_d Views.up_view128 in    
+      DV.length_eq (get_downview hkeys_b);
+       let h = reverse_bytes_quad32 (low_buffer_read TUInt8 TUInt128 h1 hkeys_b 0) in
+       let length_quad = reverse_bytes_quad32 (Mkfour (8 * UInt64.v plain_len) 0 (8 * UInt64.v auth_bytes) 0) in
+       let auth_d = get_downview auth_b in
+       length_aux3 auth_b (UInt64.v auth_num);
+       let auth_u = UV.mk_buffer auth_d Views.up_view128 in
+       let abytes_d = get_downview abytes_b in
+       length_aux3 abytes_b 1;      
+       let abytes_u = UV.mk_buffer abytes_d Views.up_view128 in        
+       let cipher_bytes =
+         if UInt64.v plain_len > (UInt64.v len128x6' + UInt64.v len128_num') * 128/8 then
+           UV.as_seq h1 inout_u
+         else Seq.empty
+       in let auth_in =
+         if UInt64.v auth_bytes > UInt64.v auth_num * 128 / 8 then
+           Seq.append (Seq.append (Seq.append (Seq.append (Seq.append
+             (UV.as_seq h0 auth_u) (UV.as_seq h0 abytes_u))
+             (UV.as_seq h1 out128x6_u))
+             (UV.as_seq h1 out128_u))
+             cipher_bytes)
+             (Seq.create 1 length_quad)
+         else
+           Seq.append (Seq.append (Seq.append (Seq.append
+             (UV.as_seq h0 auth_u) (UV.as_seq h1 out128x6_u))
+             (UV.as_seq h1 out128_u))
+             cipher_bytes)
+             (Seq.create 1 length_quad)
+       in
+       DV.length_eq (get_downview tag_b);
+       low_buffer_read TUInt8 TUInt128 h1 tag_b 0 ==
+         gctr_encrypt_block ctr_BE_1 (ghash_LE h auth_in) AES_128 (Ghost.reveal key) 0
+         );
+
+    // Need to prove that seq append commutes…
+    assume (
+      length_aux4 iv_b;
+       DV.length_eq (get_downview iv_b);
+       let iv_LE = low_buffer_read TUInt8 TUInt128 h0 iv_b 0 in
+       let iv_BE = reverse_bytes_quad32 iv_LE in
+       let ctr_BE_1 = Mkfour 1 iv_BE.lo1 iv_BE.hi2 iv_BE.hi3 in    
+       let out128x6_d = get_downview out128x6_b in
+       length_aux3 out128x6_b (UInt64.v len128x6');
+       let out128x6_u = UV.mk_buffer out128x6_d Views.up_view128 in
+       let out128_d = get_downview out128_b in
+       length_aux3 out128_b (UInt64.v len128_num');
+       let out128_u = UV.mk_buffer out128_d Views.up_view128 in      
+       let inout_d = get_downview inout_b in
+       length_aux3 inout_b 1;      
+       let inout_u = UV.mk_buffer inout_d Views.up_view128 in    
+      DV.length_eq (get_downview hkeys_b);
+       let h = reverse_bytes_quad32 (low_buffer_read TUInt8 TUInt128 h1 hkeys_b 0) in
+       let length_quad = reverse_bytes_quad32 (Mkfour (8 * UInt64.v plain_len) 0 (8 * UInt64.v auth_bytes) 0) in
+       let auth_d = get_downview auth_b in
+       length_aux3 auth_b (UInt64.v auth_num);
+       let auth_u = UV.mk_buffer auth_d Views.up_view128 in
+       let abytes_d = get_downview abytes_b in
+       length_aux3 abytes_b 1;      
+       let abytes_u = UV.mk_buffer abytes_d Views.up_view128 in        
+       let cipher_bytes =
+         if UInt64.v plain_len > (UInt64.v len128x6' + UInt64.v len128_num') * 128/8 then
+           UV.as_seq h1 inout_u
+         else Seq.empty in
+       let out_d = get_downview out_b in
+       length_aux3 out_b (UInt64.v plain_len / 16); 
+       DV.length_eq (get_downview out_b);
+       let out_u = UV.mk_buffer out_d Views.up_view128 in         
+    Seq.equal
+      (Seq.append (Seq.append (Seq.append (Seq.append (Seq.append
+             (UV.as_seq h0 auth_u) (UV.as_seq h0 abytes_u))
+             (UV.as_seq h1 out128x6_u))
+             (UV.as_seq h1 out128_u))
+             cipher_bytes)
+             (Seq.create 1 length_quad))
+      (Seq.append (Seq.append (Seq.append (Seq.append
+             (UV.as_seq h0 auth_u) (UV.as_seq h0 abytes_u))
+             (Seq.append (UV.as_seq h1 out128x6_u) (UV.as_seq h1 out128_u)))
+             cipher_bytes)
+             (Seq.create 1 length_quad))
+          );
+
+    // Need to prove that seq append commutes…
+    assume (
+      length_aux4 iv_b;
+       DV.length_eq (get_downview iv_b);
+       let iv_LE = low_buffer_read TUInt8 TUInt128 h0 iv_b 0 in
+       let iv_BE = reverse_bytes_quad32 iv_LE in
+       let ctr_BE_1 = Mkfour 1 iv_BE.lo1 iv_BE.hi2 iv_BE.hi3 in    
+       let out128x6_d = get_downview out128x6_b in
+       length_aux3 out128x6_b (UInt64.v len128x6');
+       let out128x6_u = UV.mk_buffer out128x6_d Views.up_view128 in
+       let out128_d = get_downview out128_b in
+       length_aux3 out128_b (UInt64.v len128_num');
+       let out128_u = UV.mk_buffer out128_d Views.up_view128 in      
+       let inout_d = get_downview inout_b in
+       length_aux3 inout_b 1;      
+       let inout_u = UV.mk_buffer inout_d Views.up_view128 in    
+      DV.length_eq (get_downview hkeys_b);
+       let h = reverse_bytes_quad32 (low_buffer_read TUInt8 TUInt128 h1 hkeys_b 0) in
+       let length_quad = reverse_bytes_quad32 (Mkfour (8 * UInt64.v plain_len) 0 (8 * UInt64.v auth_bytes) 0) in
+       let auth_d = get_downview auth_b in
+       length_aux3 auth_b (UInt64.v auth_num);
+       let auth_u = UV.mk_buffer auth_d Views.up_view128 in
+       let abytes_d = get_downview abytes_b in
+       length_aux3 abytes_b 1;      
+       let abytes_u = UV.mk_buffer abytes_d Views.up_view128 in        
+       let cipher_bytes =
+         if UInt64.v plain_len > (UInt64.v len128x6' + UInt64.v len128_num') * 128/8 then
+           UV.as_seq h1 inout_u
+         else Seq.empty in
+       let out_d = get_downview out_b in
+       length_aux3 out_b (UInt64.v plain_len / 16); 
+       DV.length_eq (get_downview out_b);
+       let out_u = UV.mk_buffer out_d Views.up_view128 in         
+    Seq.equal
+      (Seq.append (Seq.append (Seq.append (Seq.append
+             (UV.as_seq h0 auth_u)
+             (UV.as_seq h1 out128x6_u))
+             (UV.as_seq h1 out128_u))
+             cipher_bytes)
+             (Seq.create 1 length_quad))
+      (Seq.append (Seq.append (Seq.append
+             (UV.as_seq h0 auth_u) 
+             (Seq.append (UV.as_seq h1 out128x6_u) (UV.as_seq h1 out128_u)))
+             cipher_bytes)
+             (Seq.create 1 length_quad))
+          );
+
+
+    assume ((UInt64.v len128x6' + UInt64.v len128_num') * 128/8 = B.length plain_b);
+    assume (UInt64.v len128x6' + UInt64.v len128_num' = B.length plain_b / 16);
+
+    lemma_uv_split h0 plain_b (uint64_to_uint32 len128x6);
+    let h1 = get() in
+    lemma_uv_split h1 out_b (uint64_to_uint32 len128x6)
 
   ) else (
     let len128x6 = 0ul in
     // Compute the size of the remaining 128-bit blocks
     let len128_num = ((plain_len / 16uL) * 16uL) in
-    let auth_num = (auth_len / 16uL) * 16uL in
     // Casting to uint32 is here the equality
     FStar.Math.Lemmas.small_mod (UInt64.v len128_num) pow2_32;
-    FStar.Math.Lemmas.small_mod (UInt64.v auth_num) pow2_32;
     let in128x6_b = B.sub plain_b 0ul len128x6 in
     let out128x6_b = B.sub out_b 0ul len128x6 in
     let in128_b = B.sub plain_b len128x6 (uint64_to_uint32 len128_num) in
     let out128_b = B.sub out_b len128x6 (uint64_to_uint32 len128_num) in
-    let vauth_b = B.sub auth_b 0ul (uint64_to_uint32 auth_num) in
+
+    let auth_num = UInt64.div auth_bytes 16uL in
+    let len128_num' = UInt64.div len128_num 16uL in
+    let len128x6' = 0uL in
 
     gcm128_encrypt_opt'
       key
-      vauth_b 
-      auth_len 
-      (UInt64.div auth_num 16uL) 
+      auth_b 
+      auth_bytes
+      auth_num
       keys_b 
       iv_b 
       hkeys_b 
       abytes_b 
       in128x6_b
       out128x6_b 
-      0uL
+      len128x6'
       in128_b
       out128_b
-      (UInt64.div len128_num 16uL)
+      len128_num'
       inout_b
       plain_len 
       scratch_b
-      tag_b
+      tag_b;
 
+    let h1 = get() in
+
+   // Need to prove that seq append commutes…
+    assume (
+      length_aux4 iv_b;
+       DV.length_eq (get_downview iv_b);
+       let iv_LE = low_buffer_read TUInt8 TUInt128 h0 iv_b 0 in
+       let iv_BE = reverse_bytes_quad32 iv_LE in
+       let ctr_BE_1 = Mkfour 1 iv_BE.lo1 iv_BE.hi2 iv_BE.hi3 in    
+       let out128x6_d = get_downview out128x6_b in
+       length_aux3 out128x6_b (UInt64.v len128x6');
+       let out128x6_u = UV.mk_buffer out128x6_d Views.up_view128 in
+       let out128_d = get_downview out128_b in
+       length_aux3 out128_b (UInt64.v len128_num');
+       let out128_u = UV.mk_buffer out128_d Views.up_view128 in      
+       let inout_d = get_downview inout_b in
+       length_aux3 inout_b 1;      
+       let inout_u = UV.mk_buffer inout_d Views.up_view128 in    
+      DV.length_eq (get_downview hkeys_b);
+       let h = reverse_bytes_quad32 (low_buffer_read TUInt8 TUInt128 h1 hkeys_b 0) in
+       let length_quad = reverse_bytes_quad32 (Mkfour (8 * UInt64.v plain_len) 0 (8 * UInt64.v auth_bytes) 0) in
+       let auth_d = get_downview auth_b in
+       length_aux3 auth_b (UInt64.v auth_num);
+       let auth_u = UV.mk_buffer auth_d Views.up_view128 in
+       let abytes_d = get_downview abytes_b in
+       length_aux3 abytes_b 1;      
+       let abytes_u = UV.mk_buffer abytes_d Views.up_view128 in        
+       let cipher_bytes =
+         if UInt64.v plain_len > (UInt64.v len128x6' + UInt64.v len128_num') * 128/8 then
+           UV.as_seq h1 inout_u
+         else Seq.empty in
+       let out_d = get_downview out_b in
+       length_aux3 out_b (UInt64.v plain_len / 16); 
+       DV.length_eq (get_downview out_b);
+       let out_u = UV.mk_buffer out_d Views.up_view128 in         
+    Seq.equal
+      (Seq.append (Seq.append (Seq.append (Seq.append (Seq.append
+             (UV.as_seq h0 auth_u) (UV.as_seq h0 abytes_u))
+             (UV.as_seq h1 out128x6_u))
+             (UV.as_seq h1 out128_u))
+             cipher_bytes)
+             (Seq.create 1 length_quad))
+      (Seq.append (Seq.append (Seq.append (Seq.append
+             (UV.as_seq h0 auth_u) (UV.as_seq h0 abytes_u))
+             (Seq.append (UV.as_seq h1 out128x6_u) (UV.as_seq h1 out128_u)))
+             cipher_bytes)
+             (Seq.create 1 length_quad))
+          );
+
+    // Need to prove that seq append commutes…
+    assume (
+      length_aux4 iv_b;
+       DV.length_eq (get_downview iv_b);
+       let iv_LE = low_buffer_read TUInt8 TUInt128 h0 iv_b 0 in
+       let iv_BE = reverse_bytes_quad32 iv_LE in
+       let ctr_BE_1 = Mkfour 1 iv_BE.lo1 iv_BE.hi2 iv_BE.hi3 in    
+       let out128x6_d = get_downview out128x6_b in
+       length_aux3 out128x6_b (UInt64.v len128x6');
+       let out128x6_u = UV.mk_buffer out128x6_d Views.up_view128 in
+       let out128_d = get_downview out128_b in
+       length_aux3 out128_b (UInt64.v len128_num');
+       let out128_u = UV.mk_buffer out128_d Views.up_view128 in      
+       let inout_d = get_downview inout_b in
+       length_aux3 inout_b 1;      
+       let inout_u = UV.mk_buffer inout_d Views.up_view128 in    
+      DV.length_eq (get_downview hkeys_b);
+       let h = reverse_bytes_quad32 (low_buffer_read TUInt8 TUInt128 h1 hkeys_b 0) in
+       let length_quad = reverse_bytes_quad32 (Mkfour (8 * UInt64.v plain_len) 0 (8 * UInt64.v auth_bytes) 0) in
+       let auth_d = get_downview auth_b in
+       length_aux3 auth_b (UInt64.v auth_num);
+       let auth_u = UV.mk_buffer auth_d Views.up_view128 in
+       let abytes_d = get_downview abytes_b in
+       length_aux3 abytes_b 1;      
+       let abytes_u = UV.mk_buffer abytes_d Views.up_view128 in        
+       let cipher_bytes =
+         if UInt64.v plain_len > (UInt64.v len128x6' + UInt64.v len128_num') * 128/8 then
+           UV.as_seq h1 inout_u
+         else Seq.empty in
+       let out_d = get_downview out_b in
+       length_aux3 out_b (UInt64.v plain_len / 16); 
+       DV.length_eq (get_downview out_b);
+       let out_u = UV.mk_buffer out_d Views.up_view128 in         
+    Seq.equal
+      (Seq.append (Seq.append (Seq.append (Seq.append
+             (UV.as_seq h0 auth_u)
+             (UV.as_seq h1 out128x6_u))
+             (UV.as_seq h1 out128_u))
+             cipher_bytes)
+             (Seq.create 1 length_quad))
+      (Seq.append (Seq.append (Seq.append
+             (UV.as_seq h0 auth_u) 
+             (Seq.append (UV.as_seq h1 out128x6_u) (UV.as_seq h1 out128_u)))
+             cipher_bytes)
+             (Seq.create 1 length_quad))
+          );
+
+    assume ((UInt64.v len128x6' + UInt64.v len128_num') * 128/8 = B.length plain_b);
+    assume (UInt64.v len128x6' + UInt64.v len128_num' = B.length plain_b / 16);
+
+    lemma_uv_split h0 plain_b len128x6;
+    
+    // Direct postcondition of lemma_uv_split, but needs to be asserted 
+    assert (
+       let in128x6_d = get_downview in128x6_b in
+       length_aux3 in128x6_b (UInt64.v len128x6');
+       let in128x6_u = UV.mk_buffer in128x6_d Views.up_view128 in
+       let in128_d = get_downview in128_b in
+       length_aux3 in128_b (UInt64.v len128_num');
+       let in128_u = UV.mk_buffer in128_d Views.up_view128 in 
+       let in_d = get_downview plain_b in
+       length_aux3 plain_b (B.length plain_b / 16);
+       let in_u = UV.mk_buffer in_d Views.up_view128 in 
+       let split_bs = Seq.append (UV.as_seq h0 in128x6_u) (UV.as_seq h0 in128_u) in
+       let bs = UV.as_seq h0 in_u in
+       Seq.equal bs split_bs);
+
+    let h1 = get() in
+    lemma_uv_split h1 out_b len128x6;
+
+    // Direct postcondition of lemma_uv_split, but needs to be asserted
+    assert (
+       let out128x6_d = get_downview out128x6_b in
+       length_aux3 out128x6_b (UInt64.v len128x6');
+       let out128x6_u = UV.mk_buffer out128x6_d Views.up_view128 in
+       let out128_d = get_downview out128_b in
+       length_aux3 out128_b (UInt64.v len128_num');
+       let out128_u = UV.mk_buffer out128_d Views.up_view128 in 
+       let out_d = get_downview out_b in
+       length_aux3 out_b (B.length out_b / 16);
+       let out_u = UV.mk_buffer out_d Views.up_view128 in 
+       let split_bs = Seq.append (UV.as_seq h1 out128x6_u) (UV.as_seq h1 out128_u) in
+       let bs = UV.as_seq h1 out_u in
+       Seq.equal bs split_bs)
 
   )
 
+inline_for_extraction
 let gcm128_encrypt_opt_stdcall key plain_b plain_len auth_b auth_len iv_b out_b tag_b keys_b hkeys_b =
   let h0 = get() in
 
@@ -474,12 +852,12 @@ let gcm128_encrypt_opt_stdcall key plain_b plain_len auth_b auth_len iv_b out_b 
 
   gcm128_encrypt_opt_alloca
     key
-    plain_b
+    (B.sub plain_b 0ul (((uint64_to_uint32 plain_len) / 16ul) * 16ul))
     plain_len
-    auth_b 
+    (B.sub auth_b 0ul (((uint64_to_uint32 auth_len) / 16ul) * 16ul))
     auth_len 
     iv_b
-    out_b
+    (B.sub out_b 0ul (((uint64_to_uint32 plain_len) / 16ul) * 16ul))
     tag_b
     keys_b 
     hkeys_b 
@@ -490,6 +868,5 @@ let gcm128_encrypt_opt_stdcall key plain_b plain_len auth_b auth_len iv_b out_b 
 
   // Copy back the remainder in inout_b into out_b
   B.blit inout_b 0ul out_b ((uint64_to_uint32 plain_len / 16ul) * 16ul) (uint64_to_uint32 plain_len % 16ul);
-
 
   pop_frame()
